pipit2/core/Pipit.Source.Stream.fst
@@ -3,103 +3,105 @@
    Design notes and rationale: see Pipit.Source.Stream.md. *)
 module Pipit.Source.Stream
 
-module PEB = Pipit.Exp.Base
+module PR  = Pipit.Exp.Prim
+module PP  = Pipit.Exp.Pure
+module PES = Pipit.Exp.Source
 module L   = FStar.List.Tot
 
 (* ----- Builder and fresh names ------------------------------------------ *)
 
-type stream (ts: list PEB.typ) = nat -> PEB.tterm & nat
+type stream (ts: list PR.typ) = nat -> PES.tterm & nat
 
-let fresh (a: PEB.typ) (n: nat): PEB.svar & nat =
-  ({ PEB.svname = n; svty = a }, n + 1)
+let fresh (a: PR.typ) (n: nat): PES.svar & nat =
+  ({ PES.svname = n; svty = a }, n + 1)
 
-let rec fresh_vars (ts: list PEB.typ) (n: nat): list PEB.svar & nat =
+let rec fresh_vars (ts: list PR.typ) (n: nat): list PES.svar & nat =
   match ts with
   | []      -> ([], n)
   | a :: tl -> let (x, n)  = fresh a n in
                let (xs, n) = fresh_vars tl n in
                (x :: xs, n)
 
-let rec close_vars (k: nat) (xs: list PEB.svar) (body: PEB.tterm): Tot PEB.tterm (decreases xs) =
+let rec close_vars (k: nat) (xs: list PES.svar) (body: PES.tterm): Tot PES.tterm (decreases xs) =
   match xs with
   | []      -> body
-  | x :: tl -> PEB.close_rec_t k x (close_vars (k + 1) tl body)
+  | x :: tl -> PES.close_rec_t k x (close_vars (k + 1) tl body)
 
 (* ----- Meta-unwrap ------------------------------------------------------ *)
 
-let atomize (a: PEB.typ) (t: PEB.tterm) (n: nat)
-: PEB.sterm & (PEB.tterm -> PEB.tterm) & nat =
+let atomize (a: PR.typ) (t: PES.tterm) (n: nat)
+: PES.sterm & (PES.tterm -> PES.tterm) & nat =
   match t with
-  | PEB.TTuple [e] -> (e, (fun body -> body), n)
+  | PES.TTuple [e] -> (e, (fun body -> body), n)
   | _ ->
     let (x, n) = fresh a n in
-    (PEB.SVar x, (fun body -> PEB.TLet [a] t (PEB.close_rec_t 0 x body)), n)
+    (PES.SVar x, (fun body -> PES.TLet [a] t (PES.close_rec_t 0 x body)), n)
 
-let components (ts: list PEB.typ) (t: PEB.tterm) (n: nat)
-: list PEB.sterm & (PEB.tterm -> PEB.tterm) & nat =
+let components (ts: list PR.typ) (t: PES.tterm) (n: nat)
+: list PES.sterm & (PES.tterm -> PES.tterm) & nat =
   match t with
-  | PEB.TTuple es -> (es, (fun body -> body), n)
+  | PES.TTuple es -> (es, (fun body -> body), n)
   | _ ->
     let (xs, n) = fresh_vars ts n in
-    (L.map (fun (x: PEB.svar) -> PEB.SVar x) xs,
-     (fun body -> PEB.TLet ts t (close_vars 0 xs body)),
+    (L.map (fun (x: PES.svar) -> PES.SVar x) xs,
+     (fun body -> PES.TLet ts t (close_vars 0 xs body)),
      n)
 
 (* ----- Pointwise -------------------------------------------------------- *)
 
-let fvar (#a: PEB.typ) (x: PEB.svar): stream [a] =
-  fun n -> (PEB.TTuple [PEB.SVar x], n)
+let fvar (#a: PR.typ) (x: PES.svar): stream [a] =
+  fun n -> (PES.TTuple [PES.SVar x], n)
 
-let const (#a: PEB.typ) (v: PEB.pterm): stream [a] =
-  fun n -> (PEB.TTuple [PEB.SPure v], n)
+let const (#a: PR.typ) (v: PP.pterm): stream [a] =
+  fun n -> (PES.TTuple [PES.SPure v], n)
 
-let fby (#a: PEB.typ) (v: PEB.pterm) (s: stream [a]): stream [a] =
+let fby (#a: PR.typ) (v: PP.pterm) (s: stream [a]): stream [a] =
   fun n ->
     let (t, n)    = s n in
     let (e, w, n) = atomize a t n in
-    (w (PEB.TTuple [PEB.SFby v e]), n)
+    (w (PES.TTuple [PES.SFby v e]), n)
 
-let liftP (#args: list PEB.typ) (#result: PEB.typ)
-    (p: PEB.pterm) (s: stream args): stream [result] =
+let liftP (#args: list PR.typ) (#result: PR.typ)
+    (p: PR.prim) (s: stream args): stream [result] =
   fun n ->
     let (t, n)     = s n in
     let (es, w, n) = components args t n in
-    (w (PEB.TTuple [PEB.SPureApp p es]), n)
+    (w (PES.TTuple [PES.SPureApp p es]), n)
 
 (* ----- Tupling ---------------------------------------------------------- *)
 
-let zips (#xs #ys: list PEB.typ) (x: stream xs) (y: stream ys): stream (L.append xs ys) =
+let zips (#xs #ys: list PR.typ) (x: stream xs) (y: stream ys): stream (L.append xs ys) =
   fun n ->
     let (tx, n)      = x n in
     let (exs, wx, n) = components xs tx n in
     let (ty, n)      = y n in
     let (eys, wy, n) = components ys ty n in
-    (wx (wy (PEB.TTuple (L.append exs eys))), n)
+    (wx (wy (PES.TTuple (L.append exs eys))), n)
 
-let unzips (#xs #ys: list PEB.typ) (s: stream (L.append xs ys)): stream xs & stream ys =
+let unzips (#xs #ys: list PR.typ) (s: stream (L.append xs ys)): stream xs & stream ys =
   let k = L.length xs in
   ( (fun n ->
       let (t, n)     = s n in
       let (es, w, n) = components (L.append xs ys) t n in
-      (w (PEB.TTuple (fst (L.splitAt k es))), n))
+      (w (PES.TTuple (fst (L.splitAt k es))), n))
   , (fun n ->
       let (t, n)     = s n in
       let (es, w, n) = components (L.append xs ys) t n in
-      (w (PEB.TTuple (snd (L.splitAt k es))), n)) )
+      (w (PES.TTuple (snd (L.splitAt k es))), n)) )
 
-let zip2 (#a: PEB.typ) (#b: list PEB.typ)
+let zip2 (#a: PR.typ) (#b: list PR.typ)
     (x: stream [a]) (y: stream b): stream (a :: b) =
   zips x y
 
-let zip3 (#a #b: PEB.typ) (#c: list PEB.typ)
+let zip3 (#a #b: PR.typ) (#c: list PR.typ)
     (x: stream [a]) (y: stream [b]) (z: stream c): stream (a :: b :: c) =
   zips x (zips y z)
 
-let unzip2 (#a: PEB.typ) (#b: list PEB.typ)
+let unzip2 (#a: PR.typ) (#b: list PR.typ)
     (s: stream (a :: b)): stream [a] & stream b =
   unzips #[a] #b s
 
-let unzip3 (#a #b: PEB.typ) (#c: list PEB.typ)
+let unzip3 (#a #b: PR.typ) (#c: list PR.typ)
     (s: stream (a :: b :: c)): stream [a] & stream [b] & stream c =
   let (x, yz) = unzips #[a] #(b :: c) s in
   let (y, z)  = unzips #[b] #c yz in
@@ -107,36 +109,36 @@ let unzip3 (#a #b: PEB.typ) (#c: list PEB.typ)
 
 (* ----- Binding and recursion -------------------------------------------- *)
 
-let let' (#a #b: list PEB.typ)
+let let' (#a #b: list PR.typ)
     (e: stream a) (f: stream a -> stream b): stream b =
   fun n ->
     let (ev, n)    = e n in
     let (xs, n)    = fresh_vars a n in
-    let sref: stream a = (fun m -> (PEB.TTuple (L.map (fun (x: PEB.svar) -> PEB.SVar x) xs), m)) in
+    let sref: stream a = (fun m -> (PES.TTuple (L.map (fun (x: PES.svar) -> PES.SVar x) xs), m)) in
     let (bodyv, n) = f sref n in
-    (PEB.TLet a ev (close_vars 0 xs bodyv), n)
+    (PES.TLet a ev (close_vars 0 xs bodyv), n)
 
-let mu (#a: list PEB.typ) (f: stream a -> stream a): stream a =
+let mu (#a: list PR.typ) (f: stream a -> stream a): stream a =
   fun n ->
     let (xs, n)    = fresh_vars a n in
-    let sref: stream a = (fun m -> (PEB.TTuple (L.map (fun (x: PEB.svar) -> PEB.SVar x) xs), m)) in
+    let sref: stream a = (fun m -> (PES.TTuple (L.map (fun (x: PES.svar) -> PES.SVar x) xs), m)) in
     let (bodyv, n) = f sref n in
-    (PEB.TRec a (close_vars 0 xs bodyv), n)
+    (PES.TRec a (close_vars 0 xs bodyv), n)
 
-let letrec (#a #b: list PEB.typ)
+let letrec (#a #b: list PR.typ)
     (f: stream a -> stream a) (cont: stream a -> stream b): stream b =
   let' (mu f) cont
 
 (* ----- Nodes ------------------------------------------------------------ *)
 
-let node (#args #results: list PEB.typ)
+let node (#args #results: list PR.typ)
     (head: string) (s: stream args): stream results =
   fun n ->
     let (t, n)     = s n in
     let (es, w, n) = components args t n in
-    (w (PEB.TStreamApp head es), n)
+    (w (PES.TStreamApp head es), n)
 
 (* ----- Lowering --------------------------------------------------------- *)
 
-let exp_of_stream (#a: list PEB.typ) (s: stream a): PEB.tterm =
+let exp_of_stream (#a: list PR.typ) (s: stream a): PES.tterm =
   fst (s 0)
